Fix to_dataProgTheory
for the new compiler explorer's addition of a trace type

compiler/bootstrap/translation/to_dataProgScript.sml
@@ -57,10 +57,10 @@ val res = translate (source_to_modTheory.compile_exp_def);
 
 val source_to_mod_compile_exp_side_def = theorem"source_to_mod_compile_exp_side_def"
 val source_to_mod_compile_exp_side = Q.prove(
-  `(∀x y. source_to_mod_compile_exp_side x y ⇔ T) ∧
-   (∀x y. source_to_mod_compile_exps_side x y ⇔ T) ∧
-   (∀x y. source_to_mod_compile_pes_side x y ⇔ T) ∧
-   (∀x y. source_to_mod_compile_funs_side x y ⇔ T)`,
+  `(∀x y z. source_to_mod_compile_exp_side x y z ⇔ T) ∧
+   (∀x y z. source_to_mod_compile_exps_side x y z ⇔ T) ∧
+   (∀x y z. source_to_mod_compile_pes_side x y z ⇔ T) ∧
+   (∀x y z. source_to_mod_compile_funs_side x y z ⇔ T)`,
   ho_match_mp_tac source_to_modTheory.compile_exp_ind \\ rw[]
   \\ rw[Once source_to_mod_compile_exp_side_def]
   \\ rw[definition"source_to_mod_astop_to_modop_side_def"])
@@ -71,9 +71,16 @@ val _ = translate (source_to_modTheory.compile_def);
 
 val _ = translate (mod_to_conTheory.compile_def);
 
-val _ = translate (con_to_decTheory.compile_def);
+val r = translate con_to_decTheory.compile_decs_def;
+val con_to_dec_compile_decs_side_def = theorem"con_to_dec_compile_decs_side_def";
+val con_to_dec_compile_decs_side = Q.prove(
+  `∀x y z. con_to_dec_compile_decs_side x y z ⇔ T`,
+  Induct_on`z` \\ rw[Once con_to_dec_compile_decs_side_def])
+  |> update_precondition;
 
-val _ = translate (exh_reorderTheory.compile_def);
+val r = translate (con_to_decTheory.compile_def);
+
+val r = translate (exh_reorderTheory.compile_def);
 
 val exh_reorder_compile_side_def = theorem"exh_reorder_compile_side_def"
 val exh_reorder_compile_side = Q.prove(`
@@ -85,7 +92,7 @@ val exh_reorder_compile_side = Q.prove(`
   TRY(asm_exists_tac \\ rw[]) \\
   fs[Once exh_reorderTheory.compile_cons])|>update_precondition;
 
-val _ = translate (dec_to_exhTheory.compile_def);
+val r = translate (dec_to_exhTheory.compile_def);
 
 val dec_to_exh_compile_side_def = definition"dec_to_exh_compile_side_def";
 val dec_to_exh_compile_side = Q.prove(
@@ -93,8 +100,8 @@ val dec_to_exh_compile_side = Q.prove(
   rw[dec_to_exh_compile_side_def,Once exh_reorderTheory.compile_cons])
   |> update_precondition;
 
-val _ = translate (exh_to_patTheory.pure_op_op_pmatch);
-val _ = translate (exh_to_patTheory.compile_def);
+val r = translate (exh_to_patTheory.pure_op_op_pmatch);
+val r = translate (exh_to_patTheory.compile_def);
 
 local
   val ths = ml_translatorLib.eq_lemmas();
@@ -141,6 +148,9 @@ val EqualityType_CONLANG_OP_TYPE = find_equality_type_thm``CONLANG_OP_TYPE``
 val EqualityType_PATLANG_OP_TYPE = find_equality_type_thm``PATLANG_OP_TYPE``
   |> SIMP_RULE std_ss [EqualityType_NUM,EqualityType_CONLANG_OP_TYPE]
 
+val EqualityType_BACKEND_COMMON_TRA_TYPE = find_equality_type_thm``BACKEND_COMMON_TRA_TYPE``
+  |> SIMP_RULE std_ss [EqualityType_NUM]
+
 val ctor_same_type_def = semanticPrimitivesTheory.ctor_same_type_def
 
 val EXHLANG_PAT_TYPE_def = theorem"EXHLANG_PAT_TYPE_def";
@@ -148,21 +158,87 @@ val EXHLANG_PAT_TYPE_ind = theorem"EXHLANG_PAT_TYPE_ind";
 
 val EXHLANG_PAT_TYPE_no_closures = Q.prove(
   `∀a b. EXHLANG_PAT_TYPE a b ⇒ no_closures b`,
-  cheat);
+  ho_match_mp_tac EXHLANG_PAT_TYPE_ind
+  \\ rw[EXHLANG_PAT_TYPE_def]
+  \\ rw[no_closures_def]
+  \\ TRY (
+    qmatch_assum_rename_tac`LIST_TYPE _ x1 y1` >>
+    qhdtm_x_assum`LIST_TYPE`mp_tac >>
+    last_x_assum mp_tac >>
+    rpt(pop_assum kall_tac) >>
+    map_every qid_spec_tac[`y1`,`x1`] >>
+    Induct >> simp[LIST_TYPE_def,PULL_EXISTS,no_closures_def] >>
+    qx_gen_tac`p` >>
+    simp[PULL_EXISTS,no_closures_def] >>
+    rw[] >>
+    METIS_TAC[EqualityType_def] ) >>
+  metis_tac[EqualityType_NUM,
+            EqualityType_AST_LIT_TYPE,
+            EqualityType_LIST_TYPE_CHAR,
+            EqualityType_def]);
 
 val EXHLANG_PAT_TYPE_types_match = Q.prove(
   `∀a b c d. EXHLANG_PAT_TYPE a b ∧ EXHLANG_PAT_TYPE c d ⇒ types_match b d`,
-  cheat);
-
-val EXHLANG_PAT_TYPE_11 = Q.prove(
-  `∀a b c d. EXHLANG_PAT_TYPE a b ∧ EXHLANG_PAT_TYPE c d ⇒ (a = c ⇔ b = d)`,
-  cheat);
+  ho_match_mp_tac EXHLANG_PAT_TYPE_ind \\
+  rw[EXHLANG_PAT_TYPE_def] \\
+  Cases_on`c` \\ fs[EXHLANG_PAT_TYPE_def,types_match_def,ctor_same_type_def] \\ rw[] \\
+  TRY (
+    qmatch_assum_rename_tac`LIST_TYPE _ x1 y1` >>
+    qhdtm_x_assum`LIST_TYPE`mp_tac >>
+    qmatch_assum_rename_tac`LIST_TYPE _ x2 y2` >>
+    qhdtm_x_assum`LIST_TYPE`mp_tac >>
+    last_x_assum mp_tac >>
+    rpt(pop_assum kall_tac) >>
+    map_every qid_spec_tac[`y2`,`x2`,`y1`,`x1`] >>
+    Induct >> simp[LIST_TYPE_def,PULL_EXISTS,types_match_def,ctor_same_type_def] >- (
+      Cases >> simp[LIST_TYPE_def,PULL_EXISTS,types_match_def,ctor_same_type_def] ) >>
+    qx_gen_tac`p` >>
+    gen_tac >> Cases >> simp[PULL_EXISTS,LIST_TYPE_def] >>
+    rw[types_match_def,ctor_same_type_def] >>
+    PROVE_TAC[EqualityType_def] ) >>
+  metis_tac[EqualityType_NUM,
+            EqualityType_AST_LIT_TYPE,
+            EqualityType_LIST_TYPE_CHAR,
+            EqualityType_def]);
 
 val EqualityType_EXHLANG_PAT_TYPE = Q.store_thm("EqualityType_EXHLANG_PAT_TYPE",
   `EqualityType EXHLANG_PAT_TYPE`,
   metis_tac[EqualityType_def,EXHLANG_PAT_TYPE_no_closures,
     EXHLANG_PAT_TYPE_types_match,EXHLANG_PAT_TYPE_11])
   |> store_eq_thm
+
+val EXHLANG_PAT_TYPE_11 = Q.prove(
+  `∀a b c d. EXHLANG_PAT_TYPE a b ∧ EXHLANG_PAT_TYPE c d ⇒ (a = c ⇔ b = d)`,
+  ho_match_mp_tac EXHLANG_PAT_TYPE_ind \\
+  rw[EXHLANG_PAT_TYPE_def] \\
+  Cases_on`c` \\ fs[EXHLANG_PAT_TYPE_def] \\ rw[EQ_IMP_THM] \\
+  TRY (
+    qmatch_assum_rename_tac`LIST_TYPE _ x y1` >>
+    qhdtm_x_assum`LIST_TYPE`mp_tac >>
+    qmatch_assum_rename_tac`LIST_TYPE _ x y2` >>
+    qhdtm_x_assum`LIST_TYPE`mp_tac >>
+    last_x_assum mp_tac >>
+    rpt(pop_assum kall_tac) >>
+    map_every qid_spec_tac[`y2`,`y1`,`x`] >>
+    Induct >> simp[LIST_TYPE_def,PULL_EXISTS] >>
+    rw[] >>
+    metis_tac[]) >>
+  TRY (
+    qmatch_assum_rename_tac`LIST_TYPE _ x1 y` >>
+    qhdtm_x_assum`LIST_TYPE`mp_tac >>
+    qmatch_assum_rename_tac`LIST_TYPE _ x2 y` >>
+    qhdtm_x_assum`LIST_TYPE`mp_tac >>
+    last_x_assum mp_tac >>
+    rpt(pop_assum kall_tac) >>
+    map_every qid_spec_tac[`y`,`x1`,`x2`] >>
+    Induct >> simp[LIST_TYPE_def,PULL_EXISTS] >- (
+      Cases \\ rw[LIST_TYPE_def] ) \\
+    gen_tac \\ Cases \\ rw[LIST_TYPE_def] >>
+    metis_tac[]) >>
+  metis_tac[EqualityType_NUM,
+            EqualityType_AST_LIT_TYPE,
+            EqualityType_LIST_TYPE_CHAR,
+            EqualityType_def]);
 
 val PATLANG_EXP_TYPE_def = theorem"PATLANG_EXP_TYPE_def";
 val PATLANG_EXP_TYPE_ind = theorem"PATLANG_EXP_TYPE_ind";
@@ -183,6 +259,7 @@ val PATLANG_EXP_TYPE_no_closures = Q.prove(
     rw[] >>
     METIS_TAC[EqualityType_def] ) >>
   metis_tac[EqualityType_NUM,
+            EqualityType_BACKEND_COMMON_TRA_TYPE,
             EqualityType_MODLANG_OP_TYPE,
             EqualityType_CONLANG_OP_TYPE,
             EqualityType_PATLANG_OP_TYPE,
@@ -209,6 +286,7 @@ val PATLANG_EXP_TYPE_types_match = Q.prove(
     rw[types_match_def,ctor_same_type_def] >>
     PROVE_TAC[EqualityType_def] ) >>
   metis_tac[EqualityType_NUM,
+            EqualityType_BACKEND_COMMON_TRA_TYPE,
             EqualityType_MODLANG_OP_TYPE,
             EqualityType_CONLANG_OP_TYPE,
             EqualityType_PATLANG_OP_TYPE,
@@ -244,6 +322,7 @@ val PATLANG_EXP_TYPE_11 = Q.prove(
     gen_tac \\ Cases \\ rw[LIST_TYPE_def] >>
     metis_tac[]) >>
   metis_tac[EqualityType_NUM,
+            EqualityType_BACKEND_COMMON_TRA_TYPE,
             EqualityType_MODLANG_OP_TYPE,
             EqualityType_CONLANG_OP_TYPE,
             EqualityType_PATLANG_OP_TYPE,
@@ -255,7 +334,7 @@ val EqualityType_PATLANG_EXP_TYPE = Q.prove(
   metis_tac[EqualityType_def,PATLANG_EXP_TYPE_no_closures,PATLANG_EXP_TYPE_types_match,PATLANG_EXP_TYPE_11])
   |> store_eq_thm
 
-val _ = translate (pat_to_closTheory.compile_def);
+val r = translate (pat_to_closTheory.compile_def);
 
 val pat_to_clos_compile_side = Q.prove(`
   ∀x. pat_to_clos_compile_side x ⇔ T`,
